\documentclass[a4paper,11pt]{article}
\usepackage{amsmath,amsfonts}
\usepackage[margin=1in]{geometry}
\begin{document}
\section{Chapter 1}
$
\\
{\bf{F}}=m\ddot{r} \ \ \ \
x = r \cos \phi \ \ \ \
y = r \sin \phi \ \ \ \
r = \sqrt{x^2 + y^2} \ \ \ \
\phi = \arctan(y/x) \ \ \ \
\dot{\bf{r}} = \dot{r}\hat{\bf{r}} + r \frac{d\hat{\bf{r}}}{dt} \\
{\bf{v}} \equiv \dot{\bf{r}} = \dot{r}\hat{\bf{r}} + r \dot{phi}\hat{\bf{\phi}} \ \ \ \
v_r = \dot{r} \ \ \ \
v_{\phi} = r\dot{\phi} = r \omega \ \ \ \
{\bf{a}} \equiv \ddot{\bf{r}} = \frac{d}{dt} \dot{\bf{r}} = \frac{d}{dt}(\dot{r}\hat{\bf{r}} + r\dot{\phi}\hat{\bf{\phi}}) \\
\frac{d\hat{\bf{\phi}}}{dt} = -\dot{\phi}\hat{\bf{r}} \ \ \ \
{\bf{a}} = -r\dot{\phi}^2\hat{\bf{r}} + r \ddot{\phi} \hat{\bf{\phi}}
= -r \omega^2\hat{\bf{r}} + r \alpha \hat{{\bf{\phi}}}
\\
$
\section{Chapter 2}
$
\\
f(v) = bv + cv^2 = f_{lin} + f_{quad} \ \ \ \
b = \beta D \ \ \ \
c = \gamma D^2 \ \ \ \
\beta = 1.6 \times 10^{-4} Ns/m^2 \ \ \ \
\gamma = 0.25 Ns^2/m^4 \\
m\ddot{\bf{r}} = m{\bf{g}} - b{\bf{g}} \ \ \ \
m\dot{\bf{v}} = m{\bf{g}} - b{\bf{v}} \ \ \ \
\dot{v_x} = -kv_x \ \ \ \
v_x(t) = v_{x0}e^{-\frac{t}{\tau}} \ \ \ \
\tau = 1/k = m/b (linear) \\
x_\infty = v_{x0}\tau \ \ \ \
m\dot{v_y} = mg - bv_y \ \ \ \
v_{ter} = \frac{mg}{b} \ \ \ \
v_y(t) = v_{ter} + (v_{y0} - v_{ter})e^{-\frac{t}{\tau}} \\
R_{vac} = \frac{2v_{x0}v_{y0}}{g} \ \ \ \
R = R_{vac}\left(1 - \frac{4}{3}\frac{v_{y0}}{v_{ter}} \right) \\
m\frac{dv}{dt} = -cv^2 \ \ \ \
m\left( \frac{1}{v_0} - \frac{1}{v}\right) = -ct \ \ \ \
v(t) = \frac{v_0}{1 + cv_0t/m} = \frac{v_0}{1 + t/\tau} \ \ \ \
\tau = \frac{m}{cv_0}\\
(vertical)m\dot{v} = mg - cv^2 \ \ \ \
v_{ter} = \sqrt{\frac{mg}{c}} \ \ \ \
t = \frac{v_{ter}}{g}\arctan h \left( \frac{v}{v_{ter}}\right) \\
y = \frac{(v^2_{ter})}{g}\ln \left[\cosh\left(\frac{gt}{v_{ter}} \right)\right]\\
m\ddot{{\bf{r}}} = m{\bf{g}} - cv^2\hat{{\bf{v}}} = m{\bf{g}} - cv{\bf{v}} \ \ \ \
m\dot{v_x} = -c\sqrt{v^2_x + v^2_y} v_x \ \ \ \
m\dot{v_x} = -mg - c\sqrt{v^2_x + v^2_y} v_y \\
{\bf{F}} = q{\bf{v}} \times {\bf{B}} \ \ \ \
m\dot{v_x} = qBv_y \ \ \ \
m\dot{v_y} = =qBv_x \ \ \ \
\omega_{cyclotron} = \frac{qB}{m}\ \ \ \
\dot{v_x} = \omega v_y \ \ \ \
\dot{v_y} = -\omega v_x\\
\nu = v_x + \i v_y \ \ \ \
\dot{\nu} = i \omega \nu
\nu = A e^{i \omega t} \ \ \ \
$
\section{Chapter 3}
$
\\
m\dot{v} = -\dot{m}v_{ex} + F^{ext} \ \ \ \
{\bf{R}}_{com} = \frac{1}{M}\sum_{\alpha=1}^N m_{\alpha}{\bf{r}}_{\alpha}=\frac{m_1r_1 + . . . +m_Nr_N}{M}
{\bf{l}} = {\bf{r}} \times {\bf{p}} \ \ \ \
{\bf{l}}_{\alpha} = \sum^N_{1} r_{\alpha} \times p_{\alpha} \\
F = -\nabla U \ \ \ \
F_x = -\frac{\partial U}{partial x} ...\ \ \ \
\\
$
\section{Chapter 4}
\\
$
T = \frac{1}{2}mv^2 \ \ \ \
\Delta{T = \int^2_1 F \cdot dr = W(1->2) \ \ \ \
$
\\
\section{Chapter 5}
\\
$
L\ddot{q} + R\dot{q} + \frac{1}{C}q = 0 \ \ \ \
U = \frac{1}{2}k^2 = \frac{1}{2}kA^2\cos^2(\omega t - \delta) \ \ \ \
T = \frac{1}{2}kA^2\sin^2(\omega t - \delta) \ \ \ \
\frac{b}{m} = 2 \beta \\
\omega_0 = \sqrt{\frac{k}{m}} \ \ \ \
\ddot{x} + 2\beta\dot{x} + \omega_0^2x = 0 \ \ \ \
$
\\
\end{document}
